added lenses and more monadic awesomeness

src/Data/Fuel.v
@@ -1,16 +1,19 @@
-Require Import Data.Function.
-Require Import Data.Identity.
-Require Import Data.N.
-Require Import Data.Reader.
-Require Import Data.Option.
-Require Import Structures.Monad.
-Require Import Structures.Injection.
-Require Import Structures.MonadError.
-Require Import Structures.MonadFix.
-Require Import Structures.MonadPlus.
-Require Import Structures.MonadReader.
-Require Import Structures.Functor.
-Require Import Structures.Foldable.
+Require Import FP.Data.Function.
+Require Import FP.Data.Identity.
+Require Import FP.Data.N.
+Require Import FP.Data.Reader.
+Require Import FP.Data.Option.
+Require Import FP.Structures.Monad.
+Require Import FP.Structures.Injection.
+Require Import FP.Structures.MonadError.
+Require Import FP.Structures.MonadFix.
+Require Import FP.Structures.MonadPlus.
+Require Import FP.Structures.MonadReader.
+Require Import FP.Structures.Functor.
+Require Import FP.Structures.MonadState.
+Require Import FP.Structures.Foldable.
+Require Import FP.Structures.Peano.
+Require Import FP.Structures.MonadTrans.
 
 Import FunctionNotation.
 
@@ -18,32 +21,62 @@ Inductive fuel_t m A := FuelT { un_fuel_t : reader_t N (option_t m) A }.
 Arguments FuelT {m A} _.
 Arguments un_fuel_t {m A} _.
 
-Definition mk_fuel_t {m A} : (N -> m (option A)) -> fuel_t m A := FuelT <.> ReaderT <.> compose OptionT.
-Definition run_fuel_t {m A} (n:N) : fuel_t m A -> m (option A) := run_option_t <.> run_reader_t n <.> un_fuel_t.
-Definition fun_fuel_t {m A} : fuel_t m A -> N -> m (option A) := flip run_fuel_t.
+Section MonadTrans.
+  Definition fuel_t_lift {m} {M:Monad m} {A} : m A -> fuel_t m A :=
+    FuelT <.> lift (m:=option_t m) <.> lift (m:=m).
+End MonadTrans. 
+
+Section fuel_t_Monad.
+  Context {m} {M:Monad m}.
+
+  Definition mk_fuel_t {A} : (N -> m (option A)) -> fuel_t m A :=
+    FuelT <.> ReaderT <.> compose OptionT.
+  Definition run_fuel_t {A} (n:N) : fuel_t m A -> m (option A) :=
+    run_option_t <.> run_reader_t n <.> un_fuel_t.
+  Definition fun_fuel_t {A} : fuel_t m A -> N -> m (option A) :=
+    flip run_fuel_t.
+
+  Section MonadFix.
+    Definition fuel_t_mfix {A B}
+        (ff:(A -> fuel_t m B) -> A -> fuel_t m B) (a:A) : fuel_t m B :=
+      mk_fuel_t $ fun n =>
+        fold_mfix begin fun (f: N -> A -> m (option B)) (_n:N) (a:A) =>
+           run_fuel_t n $ ff begin fun (a:A) =>
+             mk_fuel_t $ fun (__n:N) => f _n a
+           end a
+        end n a.
+    Global Instance fuel_t_MonadFix : MonadFix (fuel_t m) :=
+      { mfix := @fuel_t_mfix }.
+  End MonadFix.
+
+  Global Instance fuel_t_reader_t_FunctorInjection
+      : FunctorInjection (fuel_t m) (reader_t N (option_t m)) :=
+    { finject := @un_fuel_t _ }.
+  Global Instance reader_t_fuel_t_FunctorInjection
+      : FunctorInjection (reader_t N (option_t m)) (fuel_t m) :=
+    { finject := @FuelT _}.
+
+  Global Instance fuel_t_Monad
+      : Monad (fuel_t m) :=
+    iso_Monad (reader_t N (option_t m)).
+  Global Instance fuel_t_MonadError {E} {ME:MonadError E m}
+      : MonadError E (fuel_t m) :=
+    iso_MonadError (reader_t N (option_t m)).
+  Global Instance fuel_t_MonadState {S} {MS:MonadState S m}
+      : MonadState S (fuel_t m) :=
+    iso_MonadState (reader_t N (option_t m)).
+  Global Instance fuel_t_MonadPlus {MP:MonadPlus m}
+      : MonadPlus (fuel_t m) :=
+    iso_MonadPlus (nMP:=reader_t_MonadPlus (MP:=option_t_MonadPlus_passthrough))
+                  (reader_t N (option_t m)).
+  Global Instance fuel_t_MonadReader {R} {MR:MonadReader R m}
+      : MonadReader R (fuel_t m) :=
+    iso_MonadReader (nMR:=reader_t_MonadReader_passthrough)
+                    (reader_t N (option_t m)).
+End fuel_t_Monad.
 
 Definition fuel := fuel_t identity.
-Definition mk_fuel {A} : (N -> option A) -> fuel A := mk_fuel_t <.> compose Identity.
-Definition run_fuel {A} : N -> fuel A -> option A := compose run_identity <.> run_fuel_t.
-
-Instance fuel_t_reader_t_FunctorInjection {m} : FunctorInjection (fuel_t m) (reader_t N (option_t m)) :=
-  { finject := @un_fuel_t _ }.
-Instance reader_t_fuel_t_FunctorInjection {m} : FunctorInjection (reader_t N (option_t m)) (fuel_t m) :=
-  { finject := @FuelT _}.
-
-Instance fuel_t_Monad {m} {M:Monad m} : Monad (fuel_t m) :=
-  iso_Monad (reader_t N (option_t m)).
-Instance fuel_t_MonadPlus {m} {M:Monad m} {MP:MonadPlus m} : MonadPlus (fuel_t m) :=
-  iso_MonadPlus (reader_t N (option_t m)).
-Instance fuel_t_MonadError {E m} {M:Monad m} {ME:MonadError E m} : MonadError E (fuel_t m) :=
-  iso_MonadError (reader_t N (option_t m)).
-Instance fuel_t_MonadReader {m} {M:Monad m} {R} {MR:MonadReader R m} : MonadReader R (fuel_t m) :=
-  iso_MonadReader (reader_t N (option_t m)) (nMR:=reader_t_MonadReader_passthrough).
-
-Definition fuel_t_mfix {m} {M:Monad m} {A B} (ff:(A -> fuel_t m B) -> A -> fuel_t m B) (a:A) : fuel_t m B :=
-  mk_fuel_t $ fun n =>
-    (fold_mfix $ fun (f:N -> A -> m (option B)) n a =>
-       run_fuel_t n $ ff (fun a => mk_fuel_t $ fun n => f n a) a)
-    n a.
-Instance fuel_t_MonadFix {m} {M:Monad m} : MonadFix (fuel_t m) :=
-  { mfix := @fuel_t_mfix _ _ }.
+Definition mk_fuel {A} : (N -> option A) -> fuel A :=
+  mk_fuel_t <.> compose Identity.
+Definition run_fuel {A} : N -> fuel A -> option A :=
+  compose run_identity <.> run_fuel_t.
