src/Data/Option.v
@@ -1,21 +1,24 @@
-Require Export Coq.Init.Datatypes.
-
-Require Import Data.FunctionPre.
-Require Import Data.Identity.
-Require Import Data.StringPre.
-Require Import Structures.Functor.
-Require Import Structures.Injection.
-Require Import Structures.Injection.
-Require Import Structures.Monad.
-Require Import Structures.MonadError.
-Require Import Structures.MonadPlus.
-Require Import Structures.MonadReader.
-Require Import Structures.MonadTrans.
-Require Import Structures.Monoid.
+Require Import FP.Data.FunctionPre.
+Require Import FP.Data.Identity.
+Require Import FP.Data.StringPre.
+Require Import FP.Structures.Functor.
+Require Import FP.Structures.Injection.
+Require Import FP.Structures.Injection.
+Require Import FP.Structures.Monad.
+Require Import FP.Structures.MonadError.
+Require Import FP.Structures.MonadPlus.
+Require Import FP.Structures.MonadReader.
+Require Import FP.Structures.MonadState.
+Require Import FP.Structures.MonadTrans.
+Require Import FP.Structures.Monoid.
+Require Import FP.Structures.Comonad.
+Require Import FP.Structures.Foldable.
+Require Import FP.Structures.Alternative.
 
 Import FunctionNotation.
 Import FunctorNotation.
 Import MonadNotation.
+Import AlternativeNotation.
 
 (* option *)
 
@@ -28,7 +31,7 @@ Definition from_option {A} (a:A) (aM:option A) : A :=
   | Some a' => a'
   end.
 
-Section MonadError.
+Section throw_msg_option.
   Context {m E} {mM:Monad m} {mE:MonadError E m} {eI:Injection string E}.
 
   Definition throw_msg_option {A} (msg:string) (xM:option A) : m A :=
@@ -36,9 +39,9 @@ Section MonadError.
     | None => throw_msg msg
     | Some x => ret x
     end.
-End MonadError.
+End throw_msg_option.
 
-Section MonadPlus.
+Section zero_option.
   Context {m} {M:Monad m} {P:MonadPlus m}.
 
   Definition zero_option {A} (xM:option A) : m A :=
@@ -46,13 +49,28 @@ Section MonadPlus.
     | None => mzero
     | Some x => ret x
     end.
-End MonadPlus.
+End zero_option.
 
-Definition monoid_option {m} {M:Monoid m} {A} (f:A -> m) (xM:option A) : m :=
-  match xM with
-  | None => gunit
-  | Some x => f x
-  end.
+Section monoid_option.
+  Context {T} {TM:Monoid T}.
+  Definition monoid_option (xM:option T) : T :=
+    match xM with
+    | None => gunit
+    | Some x => x
+    end.
+End monoid_option.
+
+Section Foldable.
+  Context {A:Type}.
+  Definition option_cofold {m} {M:Comonad m} {B}
+      (f:A -> m B -> B) (b:m B) (aM:option A) : B :=
+    match aM with
+    | None => coret b
+    | Some a => f a b
+    end.
+  Global Instance option_Foldable : Foldable A (option A) :=
+    { cofold := @option_cofold }.
+End Foldable.
 
 (* option_t *)
 
@@ -60,51 +78,59 @@ Inductive option_t m (A:Type) := OptionT { un_option_t : m (option A) }.
 Arguments OptionT {m A} _.
 Arguments un_option_t {m A} _.
 
-Definition run_option_t {m A} : option_t m A -> m (option A) := un_option_t.
-
-Section option_t.
-  Definition option_t_lift {m} {M:Monad m} {A} : m A -> option_t m A := OptionT <.> fmap Some.
+Section MonadTrans.
+  Definition option_t_lift {m} {M:Monad m} {A} : m A -> option_t m A :=
+    OptionT <.> fmap Some.
   Global Instance option_t_MonadTrans : MonadTrans option_t :=
     { lift := @option_t_lift }.
+End MonadTrans.
 
+Section option_t_Monad.
   Context {m} {M:Monad m}.
 
-  Definition option_t_ret {A} (a:A) : option_t m A := OptionT $ ret $ Some a.
-  Definition option_t_bind {A B} (aMM:option_t m A) (f:A -> option_t m B)
-      : option_t m B :=
-    OptionT $ begin
-      a <- un_option_t aMM ;;
-      match a with
-      | None => ret None
-      | Some a => un_option_t $ f a
-      end
-    end.
+  Definition run_option_t {A} : option_t m A -> m (option A) := un_option_t.
 
-  Global Instance option_t_Monad : Monad (option_t m) :=
-    { ret _A := option_t_ret
-    ; bind _A _B := option_t_bind
-    }.
+  Section Monad.
+    Definition option_t_ret {A} (a:A) : option_t m A := OptionT $ ret $ Some a.
+    Definition option_t_bind {A B}
+        (aMM:option_t m A) (f:A -> option_t m B) : option_t m B :=
+      OptionT $ begin
+        a <- un_option_t aMM ;;
+        match a with
+        | None => ret None
+        | Some a => un_option_t $ f a
+        end
+      end.
+    Global Instance option_t_Monad : Monad (option_t m) :=
+      { ret := @option_t_ret
+      ; bind := @option_t_bind
+      }.
+  End Monad.
 
-  Definition option_t_zero {A} : option_t m A := OptionT $ ret None.
-  Definition option_t_plus {A} {B} (aMM:option_t m A) (bMM:option_t m B)
-      : option_t m (A+B) :=
-    OptionT $ begin
-      a <- un_option_t aMM ;;
-      match a with
-      | None => un_option_t $ inr <$> bMM
-      | Some x => un_option_t $ inl <$> aMM
-      end
-    end.
+  Section MonadPlus.
+    Definition option_t_mzero {A} : option_t m A := OptionT $ ret None.
+    Definition option_t_mplus {A} {B}
+        (aMM:option_t m A) (bMM:option_t m B) : option_t m (A+B) :=
+      OptionT $ begin
+        a <- un_option_t aMM ;;
+        match a with
+        | None => un_option_t $ inr <$> bMM
+        | Some x => un_option_t $ inl <$> aMM
+        end
+      end.
 
-  Global Instance option_t_MonadPlus : MonadPlus (option_t m) :=
-    { mzero := @option_t_zero
-    ; mplus := @option_t_plus
-    }.
+    Global Instance option_t_MonadPlus : MonadPlus (option_t m) :=
+      { mzero := @option_t_mzero
+      ; mplus := @option_t_mplus
+      }.
+  End MonadPlus.
 
   Section MonadError.
     Context {E} {ME:MonadError E m}.
+
     Definition option_t_throw {A} : E -> option_t m A := lift <.> throw.
-    Definition option_t_catch {A} (aMM:option_t m A) : (E -> option_t m A) -> option_t m A :=
+    Definition option_t_catch {A}
+        (aMM:option_t m A) : (E -> option_t m A) -> option_t m A :=
       OptionT <.> catch (un_option_t aMM) <.> compose un_option_t.
     Global Instance option_t_MonadError : MonadError E (option_t m) :=
       { throw := @option_t_throw
@@ -114,6 +140,7 @@ Section option_t.
 
   Section MonadReader.
     Context {R} {MR:MonadReader R m}.
+
     Definition option_t_ask : option_t m R := lift ask.
     Definition option_t_local {A} (f:R -> R) : option_t m A -> option_t m A :=
       OptionT <.> local f <.> un_option_t.
@@ -122,11 +149,44 @@ Section option_t.
       ; local := @option_t_local
       }.
   End MonadReader.
-End option_t.
 
-Instance option_option_t_FunctorInjection : FunctorInjection option (option_t identity) :=
+  Section MonadState.
+    Context {S} {MS:MonadState S m}.
+
+    Definition option_t_get : option_t m S := lift get.
+    Definition option_t_put (s:S) : option_t m unit := lift $ put s.
+    Global Instance option_t_MonadState : MonadState S (option_t m) :=
+      { get := option_t_get
+      ; put := option_t_put
+      }.
+  End MonadState.
+End option_t_Monad.
+
+Instance option_option_t_FunctorInjection
+    : FunctorInjection option (option_t identity) :=
   { finject := fun _ => OptionT <.> Identity}.
-Instance option_t_option_FunctorInjection : FunctorInjection (option_t identity) option :=
+Instance option_t_option_FunctorInjection
+    : FunctorInjection (option_t identity) option :=
   { finject := fun _ => un_identity <.> un_option_t }.
 Instance option_Monad : Monad option := iso_Monad (option_t identity).
 Instance option_MonadPlus : MonadPlus option := iso_MonadPlus (option_t identity).
+
+Section MonadPlus_passthrough.
+  Context {m} {M:Monad m} {MP:MonadPlus m}.
+
+  Definition option_t_mzero_passthrough {A} : option_t m A := OptionT $ mzero.
+  Definition option_t_mplus_passthrough {A B}
+      (aMM:option_t m A) (bMM:option_t m B) : option_t m (A+B) :=
+    OptionT $ begin
+      aMbM <- un_option_t aMM <+> un_option_t bMM ;;
+      ret $
+        match aMbM with
+        | inl aM => inl <$> aM
+        | inr bM => inr <$> bM
+        end
+    end.
+  Definition option_t_MonadPlus_passthrough : MonadPlus (option_t m) :=
+    {| mzero := @option_t_mzero_passthrough
+     ; mplus := @option_t_mplus_passthrough
+    |}.
+End MonadPlus_passthrough.
