src/Data/Reader.v
@@ -1,12 +1,13 @@
-Require Import Data.FunctionPre.
+Require Import FP.Data.FunctionPre.
 
-Require Import Structures.Alternative.
-Require Import Structures.Monad.
-Require Import Structures.MonadError.
-Require Import Structures.MonadFix.
-Require Import Structures.MonadPlus.
-Require Import Structures.MonadReader.
-Require Import Structures.MonadTrans.
+Require Import FP.Structures.Alternative.
+Require Import FP.Structures.Monad.
+Require Import FP.Structures.MonadError.
+Require Import FP.Structures.MonadFix.
+Require Import FP.Structures.MonadPlus.
+Require Import FP.Structures.MonadReader.
+Require Import FP.Structures.MonadTrans.
+Require Import FP.Structures.MonadState.
 
 Import AlternativeNotation.
 Import FunctionNotation.
@@ -16,71 +17,106 @@ Inductive reader_t R (m:Type -> Type) A := ReaderT { un_reader_t : R -> m A }.
 Arguments ReaderT {R m A} _.
 Arguments un_reader_t {R m A} _ _.
 
-Definition run_reader_t {R m A} : R -> reader_t R m A -> m A := flip un_reader_t.
+Section MonadTrans.
+  Context {R:Type}.
 
-Definition reader_t_ret {R m} {M:Monad m} {A} : A -> reader_t R m A :=
-  ReaderT <.> const <.> ret.
-Definition reader_t_bind {R m} {M:Monad m} {A B}
-    (aMM:reader_t R m A) (f:A -> reader_t R m B) : reader_t R m B :=
-  ReaderT $ fun r => begin
-    a <- un_reader_t aMM r ;;
-    un_reader_t (f a) r
-  end.
-Instance reader_t_Monad {R m} {M:Monad m} : Monad (reader_t R m) :=
-  { ret := @reader_t_ret _ _ _
-  ; bind := @reader_t_bind _ _ _
-  }.
-Definition reader_t_lift {R} {m} {M:Monad m} {A} (aM:m A) : reader_t R m A :=
-  ReaderT $ fun r => aM.
-Instance reader_t_MonadTrans {R} : MonadTrans (reader_t R) :=
-  { lift  := @reader_t_lift _
-  }.
+  Definition reader_t_lift {m} {M:Monad m} {A} (aM:m A) : reader_t R m A :=
+    ReaderT $ fun r => aM.
+  Global Instance reader_t_MonadTrans : MonadTrans (reader_t R) :=
+    { lift  := @reader_t_lift }.
+End MonadTrans.
 
-Definition reader_t_ask {R m} {M:Monad m} : reader_t R m R :=
-  ReaderT $ fun r => ret r.
-Definition reader_t_local {R m} {M:Monad m} {A} (f:R -> R) (aM: reader_t R m A) : reader_t R m A :=
-  ReaderT $ fun r => un_reader_t aM (f r).
-Instance reader_t_MonadReader {R m} {M:Monad m} : MonadReader R (reader_t R m) :=
-  { ask := @reader_t_ask _ _ _
-  ; local := @reader_t_local _ _ _
-  }.
+Section reader_t.
+  Context {R:Type} {m} {M:Monad m}.
 
-Definition reader_t_ask_passthrough {R1 R2 m} {M:Monad m} {MR:MonadReader R2 m} : reader_t R1 m R2 :=
-  lift ask.
-Definition reader_t_local_passthrough {R1 R2 m} {M:Monad m} {MR:MonadReader R2 m} {A} (f:R2 -> R2) (aM:reader_t R1 m A) :=
-  ReaderT $ local f <.> un_reader_t aM.
-Definition reader_t_MonadReader_passthrough {R1 R2 m} {M:Monad m} {MR:MonadReader R2 m} : MonadReader R2 (reader_t R1 m) :=
-  {| ask := @reader_t_ask_passthrough _ _ _ _ _
-   ; local := @reader_t_local_passthrough _ _ _ _ _
-  |}.                                          
+  Definition run_reader_t {A} : R -> reader_t R m A -> m A := flip un_reader_t.
 
-Definition reader_t_mfix {R m} {M:Monad m} {MF:MonadFix m} {A B}
-    (ff:(A -> reader_t R m B) -> A -> reader_t R m B) (a:A) : reader_t R m B :=
-  let ff' (f':(A*R) -> m B) :=
-    let f (a:A) := ReaderT $ fun r => f' (a,r) in
-    uncurry $ fun (a:A) (r:R) =>
-      run_reader_t r $ ff f a
-  in
-  ReaderT $ fun r => mfix ff' (a,r).
-Instance reader_t_MonadFix {R m} {M:Monad m} {MF:MonadFix m} : MonadFix (reader_t R m) :=
-  { mfix := @reader_t_mfix _ _ _ _ }.
+  Section Monad.
+    Definition reader_t_ret {A} : A -> reader_t R m A := ReaderT <.> const <.> ret.
+    Definition reader_t_bind {A B}
+        (aMM:reader_t R m A) (f:A -> reader_t R m B) : reader_t R m B :=
+      ReaderT $ fun r => begin
+        a <- un_reader_t aMM r ;;
+        un_reader_t (f a) r
+      end.
+    Global Instance reader_t_Monad : Monad (reader_t R m) :=
+      { ret := @reader_t_ret
+      ; bind := @reader_t_bind
+      }.
+  End Monad.
 
-Definition reader_t_mzero {R m} {M:Monad m} {MP:MonadPlus m} {A} : reader_t R m A :=
-  lift mzero.
-Definition reader_t_mplus {R m} {M:Monad m} {MP:MonadPlus m} {A B} (aM:reader_t R m A) (bM:reader_t R m B) :=
-  ReaderT $ fun r => un_reader_t aM r <+> un_reader_t bM r.
-Instance reader_t_MonadPlus {R m} {M:Monad m} {MP:MonadPlus m} : MonadPlus (reader_t R m) :=
-  { mzero := @reader_t_mzero _ _ _ _
-  ; mplus := @reader_t_mplus _ _ _ _
-  }.
-      
-Definition reader_t_throw {R E m} {M:Monad m} {ME:MonadError E m} {A} : E -> reader_t R m A := lift <.> throw.
-Definition reader_t_catch {R E m} {M:Monad m} {ME:MonadError E m} {A}
-    (aM:reader_t R m A) (h:E -> reader_t R m A) : reader_t R m A :=
-  ReaderT $ fun r => catch (un_reader_t aM r) $ run_reader_t r <.> h.
-Instance reader_t_MonadError {R E m} {M:Monad m} {ME:MonadError E m} : MonadError E (reader_t R m) :=
-  { throw := @reader_t_throw _ _ _ _ _
-  ; catch := @reader_t_catch _ _ _ _ _
-  }.
-  
-  
+  Section MonadReader.
+    Definition reader_t_ask : reader_t R m R :=
+      ReaderT $ fun r => ret r.
+    Definition reader_t_local {A} (f:R -> R) (aM: reader_t R m A) : reader_t R m A :=
+      ReaderT $ fun r => un_reader_t aM (f r).
+    Global Instance reader_t_MonadReader : MonadReader R (reader_t R m) :=
+      { ask := @reader_t_ask
+      ; local := @reader_t_local
+      }.
+  End MonadReader.
+
+  Section ReaderT_passthrough.
+    Context {R2} {MR2:MonadReader R2 m}.
+
+    Definition reader_t_ask_passthrough : reader_t R m R2 := lift ask.
+    Definition reader_t_local_passthrough {A} (f:R2 -> R2) (aM:reader_t R m A) :=
+      ReaderT $ local f <.> un_reader_t aM.
+    Definition reader_t_MonadReader_passthrough : MonadReader R2 (reader_t R m) :=
+      {| ask := @reader_t_ask_passthrough
+       ; local := @reader_t_local_passthrough
+      |}.                                          
+  End ReaderT_passthrough.
+
+  Section MonadState.
+    Context {S} {MS:MonadState S m}.
+
+    Definition reader_t_get : reader_t R m S := lift get.
+    Definition reader_t_put : S -> reader_t R m unit :=lift <.> put.
+    Global Instance reader_t_MonadState : MonadState S (reader_t R m) :=
+      { get := reader_t_get
+      ; put := reader_t_put
+      }.
+  End MonadState.
+
+  Section MonadFix.
+    Context {MF:MonadFix m}.
+
+    Definition reader_t_mfix {A B}
+        (ff:(A -> reader_t R m B) -> A -> reader_t R m B) (a:A) : reader_t R m B :=
+      let ff' (f':(A*R) -> m B) :=
+        let f (a:A) := ReaderT $ fun r => f' (a,r) in
+        uncurry $ fun (a:A) (r:R) =>
+          run_reader_t r $ ff f a
+      in
+      ReaderT $ fun r => mfix ff' (a,r).
+    Global Instance reader_t_MonadFix : MonadFix (reader_t R m) :=
+      { mfix := @reader_t_mfix }.
+  End MonadFix.
+
+  Section MonadPlus.
+    Context {MP:MonadPlus m}.
+
+    Definition reader_t_mzero {A} : reader_t R m A := lift mzero.
+    Definition reader_t_mplus {A B}
+        (aM:reader_t R m A) (bM:reader_t R m B) : reader_t R m (A+B) :=
+      ReaderT $ fun r => un_reader_t aM r <+> un_reader_t bM r.
+    Global Instance reader_t_MonadPlus : MonadPlus (reader_t R m) :=
+      { mzero := @reader_t_mzero
+      ; mplus := @reader_t_mplus
+      }.
+  End MonadPlus.
+
+  Section MonadError.
+    Context {E} {ME:MonadError E m}.
+
+    Definition reader_t_throw {A} : E -> reader_t R m A := lift <.> throw.
+    Definition reader_t_catch {A}
+        (aM:reader_t R m A) (h:E -> reader_t R m A) : reader_t R m A :=
+      ReaderT $ fun r => catch (un_reader_t aM r) $ run_reader_t r <.> h.
+    Global Instance reader_t_MonadError : MonadError E (reader_t R m) :=
+      { throw := @reader_t_throw
+      ; catch := @reader_t_catch
+      }.
+  End MonadError.
+End reader_t.
