src/Data/State.v
@@ -1,49 +1,95 @@
-Require Import Data.Function.
-Require Import Data.Prod.
-Require Import Data.Type.
-Require Import Structures.Functor.
-Require Import Structures.Monad.
-Require Import Structures.Multiplicative.
-Require Import Structures.MonadState.
-Require Import Data.Identity.
+Require Import FP.Data.Function.
+Require Import FP.Data.Prod.
+Require Import FP.Data.Type.
+Require Import FP.Structures.Functor.
+Require Import FP.Structures.Monad.
+Require Import FP.Structures.Multiplicative.
+Require Import FP.Structures.MonadState.
+Require Import FP.Structures.MonadError.
+Require Import FP.Structures.MonadTrans.
+Require Import FP.Structures.MonadPlus.
+Require Import FP.Structures.Alternative.
+Require Import FP.Data.Identity.
 
 Import FunctionNotation.
 Import FunctorNotation.
 Import MonadNotation.
 Import MultiplicativeNotation.
+Import AlternativeNotation.
 
 Inductive state_t S m A := StateT { un_state_t : S -> m (A * S) }.
 Arguments StateT {S m A} _.
 Arguments un_state_t {S m A} _ _.
 
-Definition run_state_t {S m A} : S -> state_t S m A -> m (A * S) := flip un_state_t.
-Definition eval_state_t {S m A} {M:Monad m} : S -> state_t S m A -> m A := fmap fst <..> run_state_t.
-Definition exec_state_t {S m A} {M:Monad m} : S -> state_t S m A -> m S := fmap snd <..> run_state_t.
+
+Section MonadTrans.
+  Context {S:Type}.
+
+  Definition state_t_lift {m} {M:Monad m} {A} (aM:m A) : state_t S m A :=
+    StateT $ fun s => fmap (flip pair s) aM.
+  Global Instance state_t_MonadTrans : MonadTrans (state_t S) :=
+    { lift  := @state_t_lift }.
+End MonadTrans.
 
 Section state_t.
-  Context {m} {M:Monad m}.
+  Context {S:Type} {m} {M:Monad m}.
 
-  Definition state_t_ret {S A} (a:A) : state_t S m A := StateT $ fun s => ret (a,s).
-  Definition state_t_bind {S A B} (aM:state_t S m A) (f:A -> state_t S m B) : state_t S m B :=
+  Definition run_state_t {A} : S -> state_t S m A -> m (A * S) := flip un_state_t.
+  Definition eval_state_t {A} : S -> state_t S m A -> m A := fmap fst <..> run_state_t.
+  Definition exec_state_t {A} : S -> state_t S m A -> m S := fmap snd <..> run_state_t.
+
+  Definition state_t_ret {A} (a:A) : state_t S m A := StateT $ fun s => ret (a,s).
+  Definition state_t_bind {A B} (aM:state_t S m A) (f:A -> state_t S m B) : state_t S m B :=
     StateT $ fun s => begin
       as' <- un_state_t aM s ;;
       let (a,s') := as' in
       un_state_t (f a) s'
     end.
-  Global Instance state_t_Monad {S} : Monad (state_t S m) :=
-    { ret := @state_t_ret _
-    ; bind := @state_t_bind _
+  Global Instance state_t_Monad : Monad (state_t S m) :=
+    { ret := @state_t_ret 
+    ; bind := @state_t_bind 
     }.
 
-  Definition state_t_get {S} : state_t S m S :=
+  Definition state_t_get : state_t S m S :=
     StateT $ fun s => ret (s,s).
-  Definition state_t_put {S} (s:S) : state_t S m unit :=
+  Definition state_t_put (s:S) : state_t S m unit :=
     StateT $ fun _ => ret (tt,s).
-  Global Instance state_t_MonadState {S} : MonadState S (state_t S m) :=
-    { get := @state_t_get _
-    ; put := @state_t_put _
+  Global Instance state_t_MonadState : MonadState S (state_t S m) :=
+    { get := @state_t_get
+    ; put := @state_t_put
     }.
-  
+
+  Section MonadError.
+    Context {E} {ME:MonadError E m}.
+
+    Definition state_t_throw {A} : E -> state_t S m A := lift <.> throw.
+    Definition state_t_catch {A}
+        (aM:state_t S m A) (h:E -> state_t S m A) : state_t S m A :=
+      StateT $ fun s => catch (un_state_t aM s) $ run_state_t s <.> h.
+    Global Instance state_t_MonadError : MonadError E (state_t S m) :=
+      { throw := @state_t_throw
+      ; catch := @state_t_catch
+      }.
+  End MonadError.
+
+  Section MonadPlus.
+    Context {MP:MonadPlus m}.
+
+    Definition state_t_mzero {A} : state_t S m A := lift mzero.
+    Definition state_t_mplus {A B}
+        (aM:state_t S m A) (bM:state_t S m B) : state_t S m (A+B) :=
+      StateT $ fun s =>
+        r <- un_state_t aM s <+> un_state_t bM s ;;
+        ret $
+          match r with
+          | inl (a,s) => (inl a,s)
+          | inr (b,s) => (inr b,s)
+          end.
+    Global Instance state_t_MonadPlus : MonadPlus (state_t S m) :=
+      { mzero := @state_t_mzero
+      ; mplus := @state_t_mplus
+      }.
+  End MonadPlus.
 End state_t.
 
 Definition state S := state_t S identity.
