src/Data/Sum.v
@@ -1,21 +1,22 @@
-Require Export Data.SumPre.
+Require Export FP.Data.SumPre.
 
-Require Import Data.AsciiPre.
-Require Import Data.BoolPre.
-Require Import Data.FunctionPre.
-Require Import Data.StringPre.
-
-Require Import Relations.RelDec.
-Require Import Structures.EqDec.
-Require Import Structures.Eqv.
-Require Import Structures.Monad.
-Require Import Structures.MonadError.
-Require Import Structures.MonadFix.
-Require Import Structures.MonadPlus.
-Require Import Structures.Monoid.
-Require Import Structures.Ord.
-Require Import Structures.RelationClasses.
-Require Import Structures.Show.
+Require Import FP.Data.AsciiPre.
+Require Import FP.Data.BoolPre.
+Require Import FP.Data.FunctionPre.
+Require Import FP.Data.StringPre.
+Require Import FP.Relations.RelDec.
+Require Import FP.Structures.EqDec.
+Require Import FP.Structures.Eqv.
+Require Import FP.Structures.Monad.
+Require Import FP.Structures.MonadError.
+Require Import FP.Structures.MonadFix.
+Require Import FP.Structures.MonadPlus.
+Require Import FP.Structures.Monoid.
+Require Import FP.Structures.Ord.
+Require Import FP.Structures.RelationClasses.
+Require Import FP.Structures.Show.
+Require Import FP.Structures.Injection.
+Require Import FP.Data.Identity.
 
 Import CharNotation.
 Import EqDecNotation.
@@ -140,110 +141,97 @@ Section Type_Monoid.
     |}.
 End Type_Monoid.
 
-Section sum_Monad.
-  Context {A:Type}.
-  Definition sum_ret {B} : B -> A+B := inr.
-  Definition sum_bind {B C} (bM:A+B) (f:B -> A+C) : A+C :=
-    match bM with
-    | inl x => inl x
-    | inr y => f y
-    end.
-  Global Instance sum_Monad : Monad (sum A) :=
-    { ret := @sum_ret
-    ; bind := @sum_bind
-    }.
-End sum_Monad.
-
-Section sum_MonadError.
-  Context {A:Type}.
-  Definition sum_throw {B} : A -> A+B := inl.
-  Definition sum_catch {B} (bM:A+B) (h:A -> A+B) : A+B :=
-    match bM with
-    | inl x => h x
-    | inr y => inr y
-    end.
-  Global Instance sum_MonadError : MonadError A (sum A) :=
-    { throw := @sum_throw
-    ; catch := @sum_catch
-    }.
-End sum_MonadError.
-       
 Inductive sum_t A m B := SumT { un_sum_t : m (A+B) }.
 Arguments SumT {A m B} un_sum_t.
 Arguments un_sum_t {A m B} _.
 
-Definition run_sum_t {A m B} : sum_t A m B -> m (A+B) := un_sum_t.
-
 Section sum_t_Monad.
   Context {A:Type} {m} {M:Monad m}.
 
-  Definition sum_t_ret {B} : B -> sum_t A m B := SumT <.> ret <.> inr.
-  Definition sum_t_bind {B C} (bMM:sum_t A m B) (f:B -> sum_t A m C) : sum_t A m C :=
-    SumT $ begin
-      ab <- un_sum_t bMM ;;
-      match ab with
-      | inl x => ret $ inl x
-      | inr y => un_sum_t $ f y
-      end
-    end.
-  Global Instance sum_t_Monad : Monad (sum_t A m) :=
-    { ret := @sum_t_ret
-    ; bind := @sum_t_bind
-    }.
+  Definition run_sum_t {B} : sum_t A m B -> m (A+B) := un_sum_t.
+
+  Section Monad.
+    Definition sum_t_ret {B} : B -> sum_t A m B := SumT <.> ret <.> inr.
+    Definition sum_t_bind {B C}
+        (bMM:sum_t A m B) (f:B -> sum_t A m C) : sum_t A m C :=
+      SumT $ begin
+        ab <- un_sum_t bMM ;;
+        match ab with
+        | inl x => ret $ inl x
+        | inr y => un_sum_t $ f y
+        end
+      end.
+    Global Instance sum_t_Monad : Monad (sum_t A m) :=
+      { ret := @sum_t_ret
+      ; bind := @sum_t_bind
+      }.
+  End Monad.
+
+  Section MonadError.
+    Definition sum_t_throw {B} : A -> sum_t A m B := SumT <.> ret <.> inl.
+    Definition sum_t_catch {B}
+        (bMM:sum_t A m B) (h:A -> sum_t A m B) : sum_t A m B :=
+      SumT $ begin
+        ab <-  un_sum_t bMM ;;
+        match ab with
+        | inl x => un_sum_t $ h x
+        | inr y => ret $ inr y
+        end
+      end.
+    Global Instance sum_t_MonadError : MonadError A (sum_t A m) :=
+      { throw := @sum_t_throw
+      ; catch := @sum_t_catch
+      }.
+  End MonadError.
+
+  Section MonadPlus.
+    Context {AM:Monoid A}.
+
+    Definition sum_t_mzero {B} : sum_t A m B := SumT $ ret $ inl gunit.
+    Definition sum_t_mplus {B C} (bMM:sum_t A m B) (cMM:sum_t A m C)
+        : sum_t A m (B+C) :=
+      SumT $ begin
+        ab <- un_sum_t bMM ;;
+        match ab with
+        | inl e1 =>
+            ac <- un_sum_t cMM ;;
+            match ac with
+            | inl e2 => ret $ inl $ e1 ** e2
+            | inr c => ret $ inr $ inr c
+            end
+        | inr b => ret $ inr $ inl b
+        end
+      end.
+    Global Instance sum_t_MonadPlus : MonadPlus (sum_t A m) :=
+      { mzero := @sum_t_mzero
+      ; mplus := @sum_t_mplus
+      }.
+  End MonadPlus.
+
+  Section MonadFix.
+    Context {MF:MonadFix m}.
+
+    Definition sum_t_mfix {B C}
+        (ff:(B -> sum_t A m C) -> B -> sum_t A m C) (b:B) : sum_t A m C :=
+      let ff' (f':B -> m (A+C)) :=
+        let f := SumT <.> f' in
+        un_sum_t <.> ff f
+      in
+      SumT $ mfix ff' b.
+    Global Instance sum_t_MonadFix : MonadFix (sum_t A m) :=
+      { mfix := @sum_t_mfix }.
+  End MonadFix.
 End sum_t_Monad.
 
-Section sum_t_MonadPlus.
-  Context {A} {aM:Monoid A} {m} {mM:Monad m}.
-
-  Definition sum_t_mzero {B} : sum_t A m B := SumT $ ret $ inl gunit.
-  Definition sum_t_mplus {B C} (bMM:sum_t A m B) (cMM:sum_t A m C) : sum_t A m (B+C) :=
-    SumT $ begin
-      ab <- un_sum_t bMM ;;
-      match ab with
-      | inl e1 =>
-          ac <- un_sum_t cMM ;;
-          match ac with
-          | inl e2 => ret $ inl $ e1 ** e2
-          | inr c => ret $ inr $ inr c
-          end
-      | inr b => ret $ inr $ inl b
-      end
-    end.
-  Global Instance sum_t_MonadPlus : MonadPlus (sum_t A m) :=
-    { mzero := @sum_t_mzero
-    ; mplus := @sum_t_mplus
-    }.
-      
-    
-End sum_t_MonadPlus.
-
-Section sum_t_MonadError.
-  Context {A:Type} {m} {M:Monad m}.
-
-  Definition sum_t_throw {B} : A -> sum_t A m B := SumT <.> ret <.> inl.
-  Definition sum_t_catch {B} (bMM:sum_t A m B) (h:A -> sum_t A m B) : sum_t A m B :=
-    SumT $ begin
-      ab <-  un_sum_t bMM ;;
-      match ab with
-      | inl x => un_sum_t $ h x
-      | inr y => ret $ inr y
-      end
-    end.
-  Global Instance sum_t_MonadError : MonadError A (sum_t A m) :=
-    { throw := @sum_t_throw
-    ; catch := @sum_t_catch
-    }.
-End sum_t_MonadError.
-
-Section sum_t_MonadFix.
-  Context {A:Type} {m} {M:Monad m} {MF:MonadFix m}.
-
-  Definition sum_t_mfix {B C} (ff:(B -> sum_t A m C) -> B -> sum_t A m C) (b:B) : sum_t A m C :=
-    let ff' (f':B -> m (A+C)) :=
-      let f := SumT <.> f' in
-      un_sum_t <.> ff f
-    in
-    SumT $ mfix ff' b.
-  Global Instance sum_t_MonadFix : MonadFix (sum_t A m) :=
-    { mfix := @sum_t_mfix }.
-End sum_t_MonadFix.
+Instance sum_sum_t_FunctorInjection {A}
+    : FunctorInjection (sum A) (sum_t A identity) :=
+  { finject := fun _ => SumT <.> Identity }.
+Instance sum_t_sum_FunctorInjection {A}
+    : FunctorInjection (sum_t A identity) (sum A) :=
+  { finject := fun _ => run_identity <.> run_sum_t }.
+Instance sum_Monad {A} : Monad (sum A) := iso_Monad (sum_t A identity).
+Instance sum_MonadPlus {A} {AM:Monoid A} : MonadPlus (sum A) :=
+  iso_MonadPlus (sum_t A identity).
+Instance sum_MonadError {A} : MonadError A (sum A) :=
+  iso_MonadError (sum_t A identity).
+  
