src/Structures/MonadState.v
@@ -1,5 +1,6 @@
-Require Import Data.Function.
-Require Import Structures.Monad.
+Require Import FP.Data.Function.
+Require Import FP.Structures.Monad.
+Require Import FP.Structures.Injection.
 
 Import FunctionNotation.
 Import MonadNotation.
@@ -12,3 +13,15 @@ Class MonadState S m :=
 Definition modify {m S} {M:Monad m} {MS:MonadState S m} (f:S -> S) : m unit :=
   x <- get ;;
   put $ f x.
+
+Section iso_MonadState.
+  Variable (n:Type -> Type).
+  Context {m} {B:FunctorBijection m n} {S} {nMR:MonadState S n}.
+
+  Definition iso_MonadState_get : m S := ffrom get.
+  Definition iso_MonadState_put (s:S) : m unit := ffrom $ put s.
+  Definition iso_MonadState : MonadState S m :=
+    {| get := @iso_MonadState_get
+     ; put := @iso_MonadState_put
+    |}.
+End iso_MonadState.
