src/Data/Lens.v
@@ -1,0 +1,42 @@
+Require Import FP.Data.Store.
+Require Import FP.Data.Function.
+
+Import FunctionNotation.
+
+Inductive lens A S := Lens { un_lens : A -> store S A }.
+Arguments Lens {A S} _.
+Arguments un_lens {A S} _ _.
+
+Definition mk_lens {A S} (get:A -> S) (set:S -> A -> A) : lens A S :=
+  Lens $ fun a => Store (fun s => set s a) (get a).
+Definition iso_lens {A B} (from:B -> A) (to:A -> B) : lens A B :=
+  Lens $ Store from <.> to.
+
+Definition lcompose {A S1 S2} (lg:lens S1 S2) (lf:lens A S1) : lens A S2 :=
+  Lens $ fun a =>
+    let '(Store f s1) := un_lens lf a in
+    let '(Store g s2) := un_lens lg s1 in
+    Store (f <.> g) s2.
+Definition lfocus {A S1 S2} : lens A S1 -> lens S1 S2 -> lens A S2 :=
+  flip lcompose.
+                        
+Definition lget {A S} (l:lens A S) (a:A) : S :=
+  store_pos $ un_lens l a.
+Definition laccess {A S} : A -> lens A S -> S :=
+  flip lget.
+
+Definition lmodify {A S} (l:lens A S) (f:S -> S) : A -> A :=
+  peeks f <.> un_lens l.
+
+Definition lset {A S} (l:lens A S) (s:S) : A -> A :=
+  lmodify l (const s).
+
+Definition lupdate {A} : A -> (A -> A) -> A := apply_to.
+
+Module LensNotation.
+  Infix "'.'" := lfocus (at level 61, right associativity).
+  Infix "'|'" := laccess (at level 63, no associativity).
+  Infix "':%'" := lmodify (at level 62, no associativity).
+  Infix "':='" := lset (at level 62, no associativity).
+  Infix "':|'" := lupdate (at level 63, no associativity).
+End LensNotation.
