src/Data/Store.v
@@ -1,0 +1,25 @@
+Require Import FP.Data.Function.
+
+Import FunctionNotation.
+
+Inductive store S A := Store
+  { store_context : S -> A
+  ; store_pos : S
+  }.
+Arguments Store {S A} _ _.
+Arguments store_context {S A} _ _.
+Arguments store_pos {S A} _.
+
+(* Seek to a relative location *)
+Definition seeks {S A} (f:S -> S) (st:store S A) : store S A :=
+  let '(Store g s) := st in Store g (f s).
+
+(* Seek to an absolute location *)
+Definition seek {S A} (s:S) : store S A -> store S A := seeks $ const s.
+
+(* Peek at a relative location *)
+Definition peeks {S A} (f:S -> S) (st:store S A) : A :=
+  let '(Store g s) := st in g $ f s.
+
+(* Peek at an absolute location *)
+Definition peek {S A} (s:S) : store S A -> A := peeks $ const s.
