src/Structures/HasLens.v
@@ -1,0 +1,5 @@
+Require Import FP.Data.Lens.
+
+Class HasLens A S :=
+  { get_lens : lens A S }.
+Arguments get_lens {A} S {HasLens}.
