src/Structures/MonadPlus.v
@@ -23,8 +23,10 @@ Instance MonadPlus_Alternative m {MP:MonadPlus m} : Alternative m :=
 Section iso_MonadPlus.
   Variable (n:Type -> Type).
   Context {m} {B:FunctorBijection m n} {nMP:MonadPlus n}.
+
   Definition iso_MonadPlus_mzero {A} : m A := ffrom mzero.
-  Definition iso_MonadPlus_mplus {A B} (aM:m A) (bM:m B) : m (A+B) := ffrom $ mplus (fto aM) (fto bM).
+  Definition iso_MonadPlus_mplus {A B} (aM:m A) (bM:m B) : m (A+B) :=
+    ffrom $ mplus (fto aM) (fto bM).
   Definition iso_MonadPlus : MonadPlus m :=
     {| mzero := @iso_MonadPlus_mzero
      ; mplus := @iso_MonadPlus_mplus
